Syntax.thy
@@ -33,6 +33,8 @@ datatype ('a,'b) com =
   | Loop "('a,'b) com" ("_*" [100] 150)
   | Parallel "('a,'b) com" "('a,'b) com"  (infixr "||" 150)
   | Thread "('a,'b) com"
+  | Capture 'b "('a,'b) com"
+  | CaptureAll "('a,'b) com"
 
 
 text \<open>Ensure there is no parallelism within a program\<close>
@@ -44,10 +46,32 @@ fun local :: "('a,'b) com \<Rightarrow> bool"
     "local (c\<^sub>1 \<cdot> c\<^sub>2) = (local c\<^sub>1 \<and> local c\<^sub>2)" |
     "local (c\<^sub>1 \<sqinter> c\<^sub>2) = (local c\<^sub>1 \<and> local c\<^sub>2)" |  
     "local (c*) = (local c)" |    
+    "local (Capture _ c) = local c" |
+    "local (CaptureAll c) = local c" |
     "local _ = True"
 
+
+class state =
+  fixes merge :: "'a \<Rightarrow> 'a \<Rightarrow> 'a"
+  (* assumes "surj (\<lambda>m. merge m s)" *)
+
+fun capBasic :: "('a,'b :: state) basic \<Rightarrow> 'b \<Rightarrow> 'b \<Rightarrow> ('a,'b) basic" where
+"capBasic \<alpha> s s' = 
+  (tag \<alpha>, {m. merge m s \<in> vc \<alpha>}, {(m,m'). (merge m s, merge m' s') \<in> beh \<alpha>})"
+
+fun uncapBasic :: "'b \<Rightarrow> ('a,'b :: state) basic \<Rightarrow> ('a,'b) basic" where
+"uncapBasic s \<alpha> = 
+  (tag \<alpha>, {merge m s |m. m \<in> vc \<alpha>}, {(merge m s, merge m' s) |m m'. (m,m') \<in> beh \<alpha>})"
+
+lemma "surj f \<Longrightarrow> {f a |a. f a \<in> A} = A"
+by fast
+
+lemma "(uncapBasic s (capBasic \<alpha> s s)) = \<alpha>"
+apply auto
+oops
+
 text \<open>Identify all operations in a program\<close>
-fun basics :: "('a,'b) com \<Rightarrow> ('a,'b) basic set"
+fun basics :: "('a,'b :: state) com \<Rightarrow> ('a,'b) basic set"
   where
     "basics (Basic \<beta>) = {\<beta>}" |
     "basics (Seq c\<^sub>1 c\<^sub>2) = basics c\<^sub>1 \<union> basics c\<^sub>2" |
@@ -57,6 +81,9 @@ fun basics :: "('a,'b) com \<Rightarrow> ('a,'b) basic set"
     "basics (Parallel c\<^sub>1 c\<^sub>2) = basics c\<^sub>1 \<union> basics c\<^sub>2" |
     "basics (Loop c) = basics c" |
     "basics (Thread c) = basics c" |
+    (* "basics (Capture s c) = uncapBasic s ` basics c" | *)
+    "basics (Capture s c) = basics c" | 
+    "basics (CaptureAll c) = {}" |
     "basics _ = {}"
 
 text \<open>Shorthand for an environment step\<close>
